src/QUIC.Spec.PacketNumber.fsti
@@ -4,17 +4,14 @@ open LowParse.Spec.Base
 module U62 = QUIC.UInt62
 module U64 = FStar.UInt64
 module U32 = FStar.UInt32
-module Secret = Lib.IntTypes
+module Secret = QUIC.Secret.Int
 
 inline_for_extraction
 noextract
 type packet_number_length_t = (x: Secret.uint32 { 1 <= Secret.v x /\ Secret.v x <= 4 })
 
 inline_for_extraction
-let parse_packet_number_kind
-  (sz: packet_number_length_t)
-: Tot parser_kind
-= total_constant_size_parser_kind (Secret.v sz)
+let parse_packet_number_kind = strong_parser_kind 1 4 None
 
 (* Packet number *)
 
@@ -51,7 +48,22 @@ let packet_number_t'
 val parse_packet_number
   (last: last_packet_number_t)
   (pn_len: packet_number_length_t)
-: Tot (parser (parse_packet_number_kind pn_len) (packet_number_t' last pn_len))
+: Tot (parser parse_packet_number_kind (packet_number_t' last pn_len))
+
+inline_for_extraction
+let parse_packet_number_kind'
+  (sz: packet_number_length_t)
+: GTot parser_kind
+= total_constant_size_parser_kind (Secret.v sz)
+
+(* we cannot use this as the actual parser kind, because it is ghost,
+   relying on the actual value of pn_len. So we work around:  *)
+
+val parse_packet_number_kind'_correct
+  (last: last_packet_number_t)
+  (pn_len: packet_number_length_t)
+: Lemma
+  (parser_kind_prop (parse_packet_number_kind' pn_len) (parse_packet_number last pn_len))
 
 val serialize_packet_number
   (last: last_packet_number_t)
